Refactor.

src/dafny/beacon/ForkChoiceHelpers.dfy
@@ -14,13 +14,9 @@
 
 include "../ssz/Constants.dfy"
 include "../utils/Eth2Types.dfy"
-// include "../utils/NativeTypes.dfy"
 include "Attestations.dfy"
 include "BeaconChainTypes.dfy"
-// include "StateTransition.dfy"
 include "Helpers.dfy"
-// include "../utils/SeqHelpers.dfy"
-
 include "ForkChoiceTypes.dfy"
 
 /**
@@ -30,54 +26,93 @@ module ForkChoiceHelpers {
     
     import opened Constants
     import opened Eth2Types
-    // import opened NativeTypes
     import opened BeaconChainTypes
-    // import opened StateTransition
     import opened BeaconHelpers
     import opened Attestations
     import opened ForkChoiceTypes
-    // import opened SeqHelpers
    
+    /**
+     *  Whether an attestation is well-formed.
+     *
+     *  @param  a       An attestattion.
+     *  @param  store   A store.
+     *  @param  links   A sequence of votes.
+     */
+    predicate isValidAttestation(a : AttestationData, store: Store, links: seq<PendingAttestation>) 
+        /** Store is well-formed. */
+        requires isClosedUnderParent(store)
+        /** The head block in `a` is in the store. */
+        requires a.beacon_block_root in store.blocks.Keys
+    {
+        //  The chain from a.beacon_block_root
+        var xc := chainRoots(a.beacon_block_root, store);
+        //  ep(a)
+        var ep :=  compute_epoch_at_slot(a.slot);
+        //  LEBB(a), LE(a) in the attestation
+        var indexOfLEBB := computeEBB(xc, ep, store);
+        //  EBBS
+        var ebbs := computeAllEBBs(xc, ep, store);
+        //  Index of Last justified checkpoint in ebbs, LJ(a). in [0..ep]
+        var indexOfLJ := lastJustified(xc, ebbs, links) as Epoch;
+        assert(0 <= indexOfLJ <= ep); 
+
+        //  The target must root must the last epoch boundary pair in chain(a.beacon_block_root)
+        //  xc[indexOfLEBB] is the block root for epoch ep in chain(a.beacon_block_root)
+        a.target == CheckPoint(ep, xc[indexOfLEBB])
+        &&
+        //  The source must be the last justified pair in chain(a.beacon_block_root)
+        a.source == CheckPoint(ep - indexOfLJ, xc[ebbs[indexOfLJ]])
+    }
+
+    /**
+     *  A well-formed store is a store for which each block
+     *  with a slot > 0 has a parent in the store.
+     *  Downward closure.
+     *
+     *  @param  store   A store.
+     */
+    predicate isClosedUnderParent(store: Store) 
+    {
+        forall k :: k in store.blocks.Keys && store.blocks[k].slot > 0 ==>
+            store.blocks[k].parent_root in store.blocks.Keys
+            && store.blocks[store.blocks[k].parent_root].slot < store.blocks[k].slot
+    }
+
+    /**
+     *  A chain of blocks roots is totally ordered slot-wise, 
+     *  and the slot of last block is zero.
+     *
+     *  @param  xr      A non-empty seq of block roots.
+     *  @param  store   A store.
+     */
+    predicate isSlotDecreasingChain(xr: seq<Root>, store: Store)  
+    {
+        |xr| >= 1
+        &&
+        (forall r :: r in xr ==> r in store.blocks.Keys)
+        &&
+        store.blocks[xr[|xr| - 1]].slot == 0 
+        &&
+        forall i :: 1 <= i < |xr| ==> store.blocks[xr[i - 1]].slot > store.blocks[xr[i]].slot
+    }
+        
     /**
      *  The view defined by a block.
      *  
-     *  @param  br      A hash root of a block.
+     *  @param  br      A hash root of a block that is in the `store`.
      *  @param  store   A store (similar to the view of the validator).
-     *  @returns        The ancestors of the block `br` in  `store` with
+     *  @returns        The ancestors's roots of the block `br` in  `store` with
      *                  oldest (genesis) the last element of the result.
      */
-    // function chain(br: Root, store: Store) : seq<BeaconBlock>
-    //     requires br in store.blocks.Keys
-    //     requires forall k :: k in store.blocks.Keys && store.blocks[k].slot > 0 ==>
-    //         store.blocks[k].parent_root in store.blocks.Keys
-    //         && store.blocks[store.blocks[k].parent_root].slot < store.blocks[k].slot 
-
-    //     ensures |chain(br, store)| >= 1
-    //     ensures chain(br, store)[|chain(br, store)| - 1].slot == 0 
-    //     //  Computation always terminates as slot number decreases (well-foundedness).
-    //     decreases store.blocks[br].slot
-    // {
-    //     if ( store.blocks[br].slot == 0 ) then
-    //         //  Should be the genesis block.
-    //         [ store.blocks[br] ]
-    //     else 
-    //         [ store.blocks[br] ] + chain(store.blocks[br].parent_root, store)
-    // }
-
-    /**
-     *  Same as above but using block roots and stores instead of blocks.
-     */
     function chainRoots(br: Root, store: Store) : seq<Root>
+        /** The block root must in the store.  */
         requires br in store.blocks.Keys
-        requires forall k :: k in store.blocks.Keys && store.blocks[k].slot > 0 ==>
-            store.blocks[k].parent_root in store.blocks.Keys
-            && store.blocks[store.blocks[k].parent_root].slot < store.blocks[k].slot 
+        /** Store is well-formed. */
+        requires isClosedUnderParent(store)
 
-        ensures |chainRoots(br, store)| >= 1
-        /** All the root values collected must be in the store.blocks map. */
-        ensures forall r :: r in chainRoots(br, store) ==> r in store.blocks.Keys
-        /** The last root value id mapped to a block with slot 0. */
-        ensures store.blocks[chainRoots(br, store)[|chainRoots(br, store)| - 1]].slot == 0 
+        /** Result is a slot-decreasing chain of roots.  */
+        ensures isSlotDecreasingChain(chainRoots(br, store), store)
+
         //  Computation always terminates as slot number decreases (well-foundedness).
         decreases store.blocks[br].slot
     {
@@ -89,64 +124,52 @@ module ForkChoiceHelpers {
     }
 
     /**
-     *  Compute the first epoch boundary block.
+     *  Compute the first block root less than or equal to an epoch.
+     *  Also known as EBB in the Gasper paper.
      *
-     *  @param  xb  A sequence of blocks.
-     *  @param  e   An epoch.
-     *  @return     The index i of the first block in xb (left to right) with 
-     *              slot number less the epoch `e` slot. 
-     *  @note       We don't need the assumption that the list of blocks in `xb`
-     *              are ordered by slot number.
-     */
-    // function computeFirstEBBIndex(xb : seq<BeaconBlock>, e :  Epoch) : nat
-    //     requires |xb| >= 1
-    //     /** Last block has slot 0. */
-    //     requires xb[|xb| - 1].slot == 0 
-
-    //     /** The result is in the range of xb. */
-    //     ensures computeFirstEBBIndex(xb, e) < |xb|
-    //     /** The slot of the result is bounded. */
-    //     ensures xb[computeFirstEBBIndex(xb, e)].slot as nat <= e as nat * SLOTS_PER_EPOCH as nat 
-    //     /** The prefix of xb[..result] has slots >  e * SLOTS_PER_EPOCH. */
-    //     ensures forall j :: 0 <= j < computeFirstEBBIndex(xb, e) ==>
-    //         xb[j].slot as nat > e as nat * SLOTS_PER_EPOCH as nat
-    //     decreases xb 
-    // {
-    //     if |xb| == 1 then 
-    //         //  only one choice, must be the block with slot == 0
-    //         0
-    //     else if xb[0].slot as nat <= e as nat * SLOTS_PER_EPOCH as nat then 
-    //         //  first block isd a good one
-    //         0
-    //     else 
-    //         //  first block has too large a slot, search suffix of xb.
-    //         1 + computeFirstEBBIndex(xb[1..], e)
-    // }
-
-    /**
-     *  Compute the first epoch boundary block root.
-     *
-     *  @param  xb      A sequence of block roots.
+     *  @param  xb      A sequence of block roots, the last one with slot == 0.
      *  @param  e       An epoch.
      *  @param  store   A store.
      *  @return         The index i of the first block root in xb (left to right) with 
-     *                  slot number less the epoch `e` slot. 
+     *                  slot number less than or equal to the epoch `e`. 
      *  @note           We don't need the assumption that the list of blocks in `xb`
      *                  are ordered by slot number.
+     *  @note           LEBB(xb) is defined by computeEBB(xb, epoch(first(xb))).
+     *  
+     *  epoch   0            1            2            3            4            5  ...
+     *          |............|............|............|............|............|  ...
+     *  block   b5----------->b4---------->b3---->b2------>b1------->b0      
+     *  slot    0             64           129    191      213       264
+     *       
+     *  For any sequence xb == [..,b5], EBB(xb, 0) == (b5, 0).
+     *
+     *  Example 1. xb == [b0, b1, b2, b3, b4, b5].
+     *  if e >= 5, EBB(xb, e) == (b0, e). 
+     *  If e == 4, EBB(xb, 4) == b1 (last block in epoch 4). 
+     *  As epoch(b0) == 4, LEBB(xb) == EBB(xb, epoch(b0)) == b1.
+     *
+     *  Example 2. xb == [b4, b5].
+     *  If e >= 2, EBB(xb,e) == (b4, e). If e == 1, EBB(xb, 1) == (b4,1).
+     *  LEBB(xb) == (64, 1).
+     *  
+     *  Example 3. xb == [b2, b3, b4, b5].
+     *  If e >= 3, EBB(xb, e) == (b2, 3). 
+     *  If 1 <= e <= 2, EBB(xb, 2) == (64,e).
+     *  LEBB(xb) == (64, 1).
      */
-    function computeFirstEBBIndexFromRoots(xb : seq<Root>, e :  Epoch, store: Store) : nat
-        requires |xb| >= 1
-        requires forall r :: r in xb ==> r in store.blocks.Keys 
-        /** Last block has slot 0. */
-        requires store.blocks[xb[|xb| - 1]].slot == 0 
+    function computeEBB(xb : seq<Root>, e :  Epoch, store: Store) : nat
+
+        /** A slot decreasing chain of roots. */
+        requires isSlotDecreasingChain(xb, store)
 
         /** The result is in the range of xb. */
-        ensures computeFirstEBBIndexFromRoots(xb, e, store) < |xb|
+        ensures computeEBB(xb, e, store) < |xb|
         /** The slot of the result is bounded. */
-        ensures store.blocks[xb[computeFirstEBBIndexFromRoots(xb, e, store)]].slot as nat <= e as nat * SLOTS_PER_EPOCH as nat 
+        ensures store.blocks[xb[computeEBB(xb, e, store)]].slot as nat <= e as nat * SLOTS_PER_EPOCH as nat 
         /** The prefix of xb[..result] has slots >  e * SLOTS_PER_EPOCH. */
-        ensures forall j :: 0 <= j < computeFirstEBBIndexFromRoots(xb, e, store) ==>
+        ensures forall j :: 0 <= j < computeEBB(xb, e, store) ==>
             store.blocks[xb[j]].slot as nat > e as nat * SLOTS_PER_EPOCH as nat
+
         decreases xb 
     {
         if |xb| == 1 then 
@@ -157,259 +180,193 @@ module ForkChoiceHelpers {
             0
         else 
             //  first block has too large a slot, search suffix of xb.
-            1 + computeFirstEBBIndexFromRoots(xb[1..], e, store)
+            1 + computeEBB(xb[1..], e, store)
     }
 
     /**
-     *  Compute the subsequence of indices of epoch boundary blocks.
-     *  @param  xb  A sequence of blocks.
-     *  @param  e   An epoch.
-     *  @returns    The sequence of EBBs indices in xb from epoch e to epoch 0.
-     *  @note       We don't need the assumption that the list of blocks in `xb`
-     *              are ordered by slot number.
-     *  @note       In the Gasper paper, there is a definition of a epoch boundary pair (A, j).
-     *              If xb is a chain (e.g. view(B)), (A, j) is the j-th epoch boundary block
-     *              iff xb[computeEBBs(xb, epoch(B) - j)] == A.
-     */
-    // function computeEBBs(xb : seq<BeaconBlock>, e :  Epoch) : seq<nat>
-    //     requires |xb| >= 1
-    //     /** Last block has slot 0. */
-    //     requires xb[|xb| - 1].slot == 0 
-
-    //     /** Each epoch has a block associated to. */
-    //     ensures |computeEBBs(xb, e)| == e as nat + 1
-    //     /** The index for each epoch is in the range of xb. */
-    //     ensures forall i :: 0 <= i < e as nat + 1 ==> computeEBBs(xb, e)[i] < |xb|
-    //     /** The sequence returned is in decreasing order slot-wise. */
-    //     ensures forall i :: 1 <= i < e as nat + 1 ==> 
-    //         xb[computeEBBs(xb, e)[i - 1]].slot >= xb[computeEBBs(xb, e)[i]].slot
-    //     /** The epoch e - i boundary block has a slot less than (e - i) * SLOTS_PER_EPOCH. */
-    //     ensures forall i :: 0 <= i < e as nat + 1 
-    //         ==> xb[computeEBBs(xb, e)[i]].slot as nat <= (e as nat - i) * SLOTS_PER_EPOCH as nat 
-    //     /** The  blocks at index j less than the epoch e - i boundary block have a slot 
-    //         larger than  (e - i) * SLOTS_PER_EPOCH. */
-    //     ensures forall i :: 0 <= i < e as nat + 1 ==> 
-    //         forall j :: 0 <= j < computeEBBs(xb, e)[i] ==>
-    //         xb[j].slot as nat > (e as nat - i) * SLOTS_PER_EPOCH as nat
-
-    //     decreases e 
-    // {
-    //     //  Get the first boundary block
-    //     [computeFirstEBBIndex(xb, e)] +
-    //     (
-    //         //  if e > 0 recursive call, otherwise, terminate.
-    //         if e == 0 then 
-    //             []
-    //         else 
-    //             computeEBBs(xb, e - 1)
-    //     )
-    // }
-
-    /**
-     *  Compute the subsequence of indices of epoch boundary block roots.
-     *  @param  xb      A sequence of block roots.
+     *  The EBB for epoch 0 is the last element of `xb`.
+     *
+     *  @param  xb      A sequence of block roots, the last one with slot == 0.
      *  @param  e       An epoch.
      *  @param  store   A store.
-     *  @returns        The sequence of EBBs indices in xb from epoch e to epoch 0.
-     *  @note           We don't need the assumption that the list of blocks in `xb`
-     *                  are ordered by slot number.
-     *                  xb 
-     *                  
-     *  @note           In the Gasper paper, there is a definition of a epoch boundary pair (A, j).
-     *                  If xb is a chain (e.g. view(B)), (A, j) is the j-th epoch boundary block
-     *                  iff xb[computeEBBs(xb, j)] == A.
-     *                  In other words, let  `r == computeEBBsFromRoots(...)`.
-     *                  `r[j]` is the index in `xb` of EBB at epoch `epoch(B) - j`.
-     *  @note           LaetstEBB is the first element of the result.
      */
-    function computeEBBsFromRoots(xb : seq<Root>, e :  Epoch, store: Store) : seq<nat>
-        requires |xb| >= 1
-        requires forall r :: r in xb ==> r in store.blocks.Keys 
-        /** Last block has slot 0. */
-        requires store.blocks[xb[|xb| - 1]].slot == 0 
+    lemma {:induction xb} ebbForEpochZeroIsLast(xb : seq<Root>, e :  Epoch, store: Store)
+        /** A slot decreasing chain of roots. */
+        requires isSlotDecreasingChain(xb, store)
+
+        ensures computeEBB(xb, 0, store) == |xb| - 1
+    {   //  Because some constraints are defined within isSlotDecreasingChain
+        //  Dafny needs some minimal help for this proof.  
+        if |xb| == 1 {
+            //  Thanks Dafny
+        }
+    }
+   
+    /**
+     *  Compute all the EBBs.
+     *
+     *  @param  xb      A sequence of block roots, the last one has slot equal to 0.
+     *  @param  e       An epoch.
+     *  @param  store   A store.
+     *  @returns        The sequence of e + 1 EBBs for each epoch 0 <= e' <= e.
+     *                  Element at index 0 <= k < |computeAllEBBs()| is 
+     *                  EBB(xb, e - k).
+     *
+     *  epoch   0            1            2            3            4            5  ...
+     *          |............|............|............|............|............|  ...
+     *  block   b5----------->b4---------->b3---->b2------>b1------->b0      
+     *  slot    0             64           129    191      213       264
+     *       
+     *  For any sequence xb == [..,b5], EBB(xb, 0) == (b5, 0).
+     *
+     *  Example 1. xb == [b0, b1, b2, b3, b4, b5].
+     *  if e >= 5, EBB(xb, e) == (b0, e). 
+     *  If e == 4, EBB(xb, 4) == b1 (last block in epoch 4). 
+     *  As epoch(b0) == 4, LEBB(xb) == EBB(xb, epoch(b0)) == b1.
+     *
+     *  Example 2. xb == [b4, b5].
+     *  If e >= 2, EBB(xb,e) == (b4, e). If e == 1, EBB(xb, 1) == (b4,1).
+     *  LEBB(xb) == (64, 1).
+     *  
+     *  Example 3. xb == [b2, b3, b4, b5].
+     *  If e >= 3, EBB(xb, e) == (b2, 3). 
+     *  If 1 <= e <= 2, EBB(xb, 2) == (64,e).
+     *  LEBB(xb) == (64, 1).
+     */
+    function computeAllEBBs(xb : seq<Root>, e :  Epoch, store: Store) : seq<nat>
+        /** A slot decreasing chain of roots. */
+        requires isSlotDecreasingChain(xb, store)
 
         /** Each epoch has a block associated to. */
-        ensures |computeEBBsFromRoots(xb, e, store)| == e as nat + 1
+        ensures |computeAllEBBs(xb, e, store)| == e as nat + 1
         /** The index for each epoch is in the range of xb. */
-        ensures forall i :: 0 <= i < e as nat + 1 ==> computeEBBsFromRoots(xb, e, store)[i] < |xb|
+        ensures forall i :: 0 <= i < e as nat + 1 ==> computeAllEBBs(xb, e, store)[i] < |xb|
         /** The sequence returned is in decreasing order slot-wise. */
         ensures forall i :: 1 <= i < e as nat + 1 ==> 
-            store.blocks[xb[computeEBBsFromRoots(xb, e, store)[i - 1]]].slot >= store.blocks[xb[computeEBBsFromRoots(xb, e, store)[i]]].slot
+            store.blocks[xb[computeAllEBBs(xb, e, store)[i - 1]]].slot >= store.blocks[xb[computeAllEBBs(xb, e, store)[i]]].slot
         /** The epoch e - i boundary block has a slot less than (e - i) * SLOTS_PER_EPOCH. */
         ensures forall i :: 0 <= i < e as nat + 1 
-            ==> store.blocks[xb[computeEBBsFromRoots(xb, e, store)[i]]].slot as nat <= (e as nat - i) * SLOTS_PER_EPOCH as nat 
+            ==> store.blocks[xb[computeAllEBBs(xb, e, store)[i]]].slot as nat <= (e as nat - i) * SLOTS_PER_EPOCH as nat 
         /** The  blocks at index j less than the epoch e - i boundary block have a slot 
             larger than  (e - i) * SLOTS_PER_EPOCH. */
         ensures forall i :: 0 <= i < e as nat + 1 ==> 
-            forall j :: 0 <= j < computeEBBsFromRoots(xb, e, store)[i] ==>
+            forall j :: 0 <= j < computeAllEBBs(xb, e, store)[i] ==>
             store.blocks[xb[j]].slot as nat > (e as nat - i) * SLOTS_PER_EPOCH as nat
+        ensures computeAllEBBs(xb, e, store)[|computeAllEBBs(xb, e, store)| - 1] == |xb| - 1
 
         decreases e 
     {
-        //  Get the first boundary block
-        [computeFirstEBBIndexFromRoots(xb, e, store)] +
+        ebbForEpochZeroIsLast(xb, e, store);
+        //  Get the first boundary block less than or equal to e
+        [computeEBB(xb, e, store)] +
         (
             //  if e > 0 recursive call, otherwise, terminate.
             if e == 0 then 
                 []
             else 
-                computeEBBsFromRoots(xb, e - 1, store)
+                computeAllEBBs(xb, e - 1, store)
         )
     }
 
     /**
-     *  LEBB definition.
+     *  A checkpoint (B, j > 0) that is justified must have more then 2/3 of
+     *  ingoing votes.
      *
-     *  @param  br      A block root. Ideally the block root of an attestation.
-     *  @param  store   The current view.
-     *  @returns        The latest epoch boudasry block for `br`.
+     *  @param  i       An index in `ebbs`.
+     *  @param  xb      Sequence of blocks roots (last one expected to be genesis block root).
+     *  @param  ebbs    A sequence of EBB from epoch |ebbs| - 1 to 0. Last element must
+     *                  be pointing to last element of `xv`.
+     *  @param  links   The votes (attestations).
      */
-    // function latestEBB(br: Root, store: Store) :  BeaconBlock
-    //     requires br in store.blocks.Keys
-    //     requires forall k :: k in store.blocks.Keys && store.blocks[k].slot > 0 ==>
-    //         store.blocks[k].parent_root in store.blocks.Keys
-    //         && store.blocks[store.blocks[k].parent_root].slot < store.blocks[k].slot
+    lemma {:induction i} justifiedMustHaveTwoThirdIncoming(i: nat, xb : seq<Root>, ebbs: seq<nat>,  links : seq<PendingAttestation>)
+        /** i is an index in ebbs not epoch 0. Each index represent an epoch so must be unint64. */
+        requires i + 1 < |ebbs| 
+        requires |ebbs| <= 0x10000000000000000
+        /** `xb` has at least one block. */
+        requires |xb| >= 1
+        /** The last element of ebbs is the EBB at epoch 0 and should be the last block in `xb`. */
+        requires ebbs[|ebbs| - 1] == |xb| - 1
         
-    // {
-    //     //  seq of beacon blocks (ancestors of br)
-    //     var ch := chain(br, store);
-    //     var bl := store.blocks[br];
-    //     var slot := bl.slot;
-    //     var lebbIndex := computeFirstEBBIndex(ch, compute_epoch_at_slot(slot));
-    //     ch[lebbIndex]
-    // }
-
-    /**
-     *  Justification definition.
-     *  
-     *  @param  i           An index in `xv`.
-     *  @param  xv          A sequence of EBB ordered by epochs from largest (first) to 0 (last).
-     *                      Each xv[i] is an EBB for epoch i.
-     *  @param  links       The attestations with src and tgt checkpoints.
-     *  @param  refSet      A non-negative int typically the number of validators.
-     *  @returns            Whether the checkpoint `xv[i]` is justified.
-     *
-     *  @note               The difficulty (if any) here is that `xv` has blocks but
-     *                      links has attestations wich src and target that are roots.
-     *                      So we need the store and the map root --> block to make the link.  
-     *  @note               We may alternatively return the sequence of indices that 
-     *                      builds the sequence of justified checkpoints (and [] if not justified).
-     */
-    predicate isJustified(i: nat, xv : seq<CheckPoint>, links : seq<PendingAttestation>, refSet: nat) 
-        requires |xv| >= 1
-        requires i < |xv|
-        /** The checkpoints must be in decreasing order epoch-wise.  */
-        requires forall i :: 0 <= i < |xv| ==> xv[i].epoch as nat == |xv| - i 
-        /** SuperMajority link requires src.epoch < tgt.epoch. */
-        // requires forall i, j :: 0 <= i < j < |xv| ==> xv[i].epoch > xv[j].epoch
-        decreases |xv| - i 
+        /** (xb[ebbs[j]], j) is the EBB at epoch |ebbs| - j and must be an index in `xb`.  */
+        requires forall i :: 0 <= i < |ebbs| ==> ebbs[i] < |xb|
+        ensures isJustified(i, xb, ebbs, links) ==>
+            |collectAttestationsForTarget(links, CheckPoint(i as Epoch, xb[ebbs[i]]))| >= ( 2 * MAX_VALIDATORS_PER_COMMITTEE) / 3 + 1
     {
-        if i == |xv| - 1 then 
-            //  Genesis block with slot 0 is justified.
-            true
-        else 
-            //  there should be a justified block at a higher index
-            exists j {:induction j} :: i < j < |xv| - 1 && isJustified(j, xv, links, refSet) 
-                && superMajorityLink(xv[j], xv[i], links, refSet)
-    }
-
-    /**
-     *  A justified pair (B, j), j > 0 implies links has more than 2/3 validators
-     *  with target (B, j)
-     */
-    lemma foo304(i: nat, xv : seq<Root>, links : seq<PendingAttestation>) 
-        requires |xv| >= 2
-        requires i + 1 < |xv| < 0x10000000000000000
-        ensures isJustified2(i, xv, links) ==>
-            |collectAttestationsForTarget(links, CheckPoint(i as Epoch, xv[i]))| >= ( 2 * MAX_VALIDATORS_PER_COMMITTEE) / 3 + 1
-    {
-        if isJustified2(i, xv, links) {
-            assert(i < |xv| - 1);
+        if isJustified(i, xb, ebbs, links) {
+            assert(i < |ebbs| - 1);
             //  i is not last element of `xv` and cannot be epoch 0.
-            assert( exists j {:induction j} :: i < j < |xv| - 1 && isJustified2(j, xv, links) 
-                && |collectAttestationsForLink(links, CheckPoint(j as Epoch, xv[j]), CheckPoint(i as Epoch, xv[i]))| >= (2 * MAX_VALIDATORS_PER_COMMITTEE) / 3 + 1);
-            var j :|  i < j < |xv| - 1 && isJustified2(j, xv, links) && |collectAttestationsForLink(links, CheckPoint(j as Epoch, xv[j]), CheckPoint(i as Epoch, xv[i]))| >= (2 * MAX_VALIDATORS_PER_COMMITTEE) / 3 + 1;
-            assert(|collectAttestationsForLink(links, CheckPoint(j as Epoch, xv[j]), CheckPoint(i as Epoch, xv[i]))| >= (2 * MAX_VALIDATORS_PER_COMMITTEE) / 3 + 1);
-            foo500(links, CheckPoint(j as Epoch, xv[j]), CheckPoint(i as Epoch, xv[i]));
+            assert( exists j :: i < j < |ebbs| - 1 && isJustified(j, xb, ebbs, links) 
+                && |collectAttestationsForLink(links, CheckPoint(j as Epoch, xb[ebbs[j]]), CheckPoint(i as Epoch, xb[ebbs[i]]))| >= (2 * MAX_VALIDATORS_PER_COMMITTEE) / 3 + 1);
+            var j :|  i < j < |ebbs| - 1 && isJustified(j, xb, ebbs, links) && |collectAttestationsForLink(links, CheckPoint(j as Epoch, xb[ebbs[j]]), CheckPoint(i as Epoch, xb[ebbs[i]]))| >= (2 * MAX_VALIDATORS_PER_COMMITTEE) / 3 + 1;
+            assert(|collectAttestationsForLink(links, CheckPoint(j as Epoch, xb[ebbs[j]]), CheckPoint(i as Epoch, xb[ebbs[i]]))| >= (2 * MAX_VALIDATORS_PER_COMMITTEE) / 3 + 1);
+            attForTgtLargerThanLinks(links, CheckPoint(j as Epoch, xb[ebbs[j]]), CheckPoint(i as Epoch, xb[ebbs[i]]));
         }
     }
 
-    
     /**
-     *  Definition of justification.  
-     *
-     *  @param  xv      A decreasing-ordered sequence of EBBs, the last one is justified.
-     *  @param  links   The votes as attestations.
-     *  @param  refSet  A number used to check supermajority. Should the be the cardinal of
-     *                  of the set of all validators.    
-     *  @param  i       An index in `xv`.
-     *  @returns        Whether `xv[i]` is justified.  
+     *  The index of the first (left to right) justified ebb.
      */
-    predicate isJustified2(i: nat, xv : seq<Root>, links : seq<PendingAttestation>) 
-        requires |xv| >= 1
-        requires i < |xv| < 0x10000000000000000
-        // requires 1 <= |ebbs| <= |xv|
-        /** The checkpoints must be in decreasing order epoch-wise.  */
-        // requires forall i :: 0 <= i < |xv| ==> xv[i].epoch as nat == |xv| - i 
-        /** SuperMajority link requires src.epoch < tgt.epoch. */
-        // requires forall i, j :: 0 <= i < j < |xv| ==> xv[i].epoch > xv[j].epoch
-        decreases |xv| - i 
-    {
-        if i == |xv| - 1 then 
-            // Last block in the list is justified.
-            true
-        else 
-            //  there should be a justified block at a higher index `j` that is justified
-            //  and a supermajority link from `j` to `i`.
-            exists j  :: i < j < |xv| - 1 && isJustified2(j, xv, links) 
-                && |collectAttestationsForLink(links, CheckPoint(j as Epoch, xv[j]), CheckPoint(i as Epoch, xv[i]))| >= (2 * MAX_VALIDATORS_PER_COMMITTEE) / 3 + 1
-    }
+    function lastJustified(xb : seq<Root>, ebbs: seq<nat>,  links : seq<PendingAttestation>): nat
+        /** `xb` has at least one block. */
+        requires |xb| >= 1
+        requires 1 <= |ebbs| <= 0x10000000000000000
+        /** The last element of ebbs is the EBB at epoch 0 and should be the last block in `xb`. */
+        requires ebbs[|ebbs| - 1] == |xb| - 1
+        /** (xb[ebbs[j]], j) is the EBB at epoch |ebbs| - j and must be an index in `xb`.  */
+        requires forall i :: 0 <= i < |ebbs| ==> ebbs[i] < |xb|
 
-    /**
-     *  Whether at epoch j <= epoch(br), block i in chainRoot(br) is justified. 
-     */
-    // predicate isJustifiedAtEpochInChain(e : Epoch, br : Root, links : seq<PendingAttestation>, store: Store, cp: CheckPoint) 
-       
-    //     requires br in store.blocks.Keys
-    //     requires forall k :: k in store.blocks.Keys && store.blocks[k].slot > 0 ==>
-    //         store.blocks[k].parent_root in store.blocks.Keys
-    //         && store.blocks[store.blocks[k].parent_root].slot < store.blocks[k].slot 
-    //     requires cp.epoch <= e 
-    //     requires cp.root in chainRoots(br, store)
-
-    //     // requires 1 <= |ebbs| <= |xv|
-    //     /** The checkpoints must be in decreasing order epoch-wise.  */
-    //     // requires forall i :: 0 <= i < |xv| ==> xv[i].epoch as nat == |xv| - i 
-    //     /** SuperMajority link requires src.epoch < tgt.epoch. */
-    //     // requires forall i, j :: 0 <= i < j < |xv| ==> xv[i].epoch > xv[j].epoch
-    //     // decreases |xv| - i 
+        ensures lastJustified(xb, ebbs, links) < |ebbs|
+        ensures isJustified(lastJustified(xb, ebbs, links), xb, ebbs, links)
+        ensures forall i :: 0 <= i < lastJustified(xb, ebbs, links) ==> 
+            !isJustified(i, xb, ebbs, links)
+    //  R1: we can compute it, but this requires a lemma to shit a result on
+    //  isJustified(i, ebbs[1..], ...) to isJustified(1 + i, ebbs)
     // {
-    //     if cp.epoch == 0 then 
-    //         // A checkpoint with epoch zero is justified if it points to genesis_block_root 
-    //         // or equivalently slot zero.
-    //         store.blocks[cp.root].slot == 0
+    //     if isJustified(0, xb, ebbs, links) then 
+    //         // assert(isJustified(0,  xb, ebbs, links));
+    //         0
     //     else 
-    //         //  Otherwise we must find a justfied checkpoint in chain(br, store)
-    //         //  The chain of br.
-    //         var ch : seq<Root> := chainRoots(br, store);
-    //         //  The slot of br.
-    //         var sl := store.blocks[br].slot ;
-    //         //  The epoch if br
-    //         // var e := compute_epoch_at_slot(sl);
-    //         //  The indices of EBBs. ebbsIndices[j] is the index of a block in ch such 
-    //         //  that (ebbsIndices[j], e - j) is the EBB for epoch e - j
-    //         var ebbsIndices : seq<nat> := computeEBBsFromRoots(ch, e, store);
-    //         true
-    //         exists j {:induction j} :: i < j < e - 1 && isJustified2(j, xv, links, refSet) 
-    // //             && superMajorityLink(CheckPoint(j as Epoch, xv[j]), CheckPoint(i as Epoch, xv[i]), links, refSet)
-    // //     if i == |xv| - 1 then 
-    // //         // Last block in the list is justified.
-    // //         true
-    // //     else 
-    // //         //  there should be a justified block at a higher index `j` that is justified
-    // //         //  and a supermajority link from `j` to `i`.
-    // //         exists j {:induction j} :: i < j < |xv| - 1 && isJustified2(j, xv, links, refSet) 
-    // //             && superMajorityLink(CheckPoint(j as Epoch, xv[j]), CheckPoint(i as Epoch, xv[i]), links, refSet)
+    //          // use of a lemma would be needed here, see R1 above.
+    //         // assert(isJustified(1 + lastJustified(xb, ebbs[1..], links), xb, ebbs, links));
+    //         1 + lastJustified(xb, ebbs[1..], links)
     // }
 
+    /**
+     *  
+     *  @param  i       An index in the sequence of ebbs.
+     *  @param  xb      A sequence of block roots.
+     *  @param  ebbs    A sequence of indices. (xb[ebbs(j)],j) is EBB(xb, |ebbs| - 1 - j).
+     *                  The last element (xb[ebbs[|ebbs| - 1]], |ebbs| - 1 - (|ebbs| - 1) )
+     *                  i.e. (xb[|xb| - 1], 0) is assumed to be justified.
+     *  @param  links   The attestations (votes).
+     *  @returns        Whether (xb[ebbs[i]], i) is justified according to the votes in *                  `links`.         
+     *  @note           ebbs contains EBB for epochs |ebbs| - 1 down to 0. 
+     */
+    predicate isJustified(i: nat, xb : seq<Root>, ebbs: seq<nat>,  links : seq<PendingAttestation>)
+        /** i is an index in ebbs, and each index represent an epoch so must be unint64. */
+        requires i < |ebbs| <= 0x10000000000000000
+        /** `xb` has at least one block. */
+        requires |xb| >= 1
+        /** The last element of ebbs is the EBB at epoch 0 and should be the last block in `xb`. */
+        requires ebbs[|ebbs| - 1] == |xb| - 1
+        
+        /** (xb[ebbs[j]], j) is the EBB at epoch |ebbs| - j and must be an index in `xb`.  */
+        requires forall i :: 0 <= i < |ebbs| ==> ebbs[i] < |xb|
+
+        decreases |ebbs| - i 
+    {
+        // true
+        if i == |ebbs| - 1 then 
+            // Last block in the list is assumed to be justified.
+            true
+        else 
+            //  There should be a justified block at a higher index `j` that is justified
+            //  and a supermajority link from `j` to `i`.
+            exists j  :: i < j < |ebbs| - 1 && isJustified(j, xb, ebbs, links) 
+                && |collectAttestationsForLink(
+                    links, 
+                    CheckPoint(j as Epoch, xb[ebbs[j]]), 
+                    CheckPoint(i as Epoch, xb[ebbs[i]]))| 
+                        >= (2 * MAX_VALIDATORS_PER_COMMITTEE) / 3 + 1
+    }
 }
